TAPLFormalization/SemanticsTheorems.lean
@@ -1,6 +1,6 @@
 import TAPLFormalization.Semantics
 
-lemma no_step_from_NV : NumericValue t → ∀ t', ¬(t ~> t') := by
+lemma no_step_from_NV : IsNumericValue t → ∀ t', ¬(t ~> t') := by
   intro t_nv t'
   induction t_nv generalizing t' with
   | zero => intro; contradiction
@@ -11,22 +11,38 @@ lemma no_step_from_NV : NumericValue t → ∀ t', ¬(t ~> t') := by
 
 theorem smallStep_deterministic : (t₁ ~> t₂) → (t₁ ~> t₃) → (t₂ = t₃) := by
   intro st₂ st₃
-  induction t₁ generalizing t₂ t₃ <;> try contradiction
-  all_goals cases st₂ <;> cases st₃
+  induction t₁ generalizing t₂ t₃ <;> cases st₂ <;> cases st₃
   any_goals rfl
   any_goals contradiction
   -- When st₂ and st₃ are from the same constructor, we can apply (one of) ih
-  any_goals try (congr; apply_assumption <;> assumption)
-  -- Otherwise, we have a step from NV
-  all_goals grind [no_step_from_NV, NumericValue.succ]
+  any_goals (congr; apply_assumption <;> assumption)
+  -- Otherwise, we have a step t~>t', where t is an NV -- contradiction
+  all_goals grind [no_step_from_NV, IsNumericValue]
 
 def isNF (t : Term) := ∀ (t' : Term), ¬(t ~> t')
 
-theorem boolean_isNF_iff_isValue : ∀ (t : Term), BooleanTerm t → (isNF t ↔ Value t) := by
-  sorry
+theorem isNF_if_isValue : ∀ (t : Term),  IsValue t → isNF t := by
+  intro t t_value t' bad_step
+  cases t_value <;> try contradiction
+  rename_i t_nv
+  exact no_step_from_NV t_nv t' bad_step
 
-theorem isNF_if_isValue : ∀ (t : Term),  Value t → isNF t := by
-  sorry
+theorem boolean_isNF_iff_isValue : ∀ (t : Term), BooleanTerm t → (isNF t ↔ IsValue t) := by
+  intro t t_boolean
+  apply Iff.intro
+  · intro t_nf
+    cases t_boolean <;> try constructor
+    rename_i t₁ t₂ t₃ t₁_boolean t₂_boolean t₃_boolean
+    suffices h : False by contradiction
+    induction t₁_boolean generalizing t₂ t₃
+    · exact t_nf t₂ .IfTrue
+    · exact t_nf t₃ .IfFalse
+    · rename_i t₁₁ t₁₂ t₁₃ t₁₁_boolean t₁₂_boolean t₁₃_boolean ih₁ ih₂ ih₃
+      let t₁_not_NF := Not.intro $ ih₁ t₁₂_boolean t₁₃_boolean
+      rw [isNF, Classical.not_forall_not] at t₁_not_NF
+      let ⟨t', st⟩ := t₁_not_NF
+      exact t_nf _ (.If st)
+  · exact isNF_if_isValue t
 
 theorem NF_unique (tu : t ~>* u) (tu' : t ~>* u') (nfu : isNF u) (nfu' : isNF u') : u = u' := by
   induction tu with
@@ -49,4 +65,22 @@ theorem NF_unique (tu : t ~>* u) (tu' : t ~>* u') (nfu : isNF u) (nfu' : isNF u'
       exact ih
 
 theorem termination : ∀ (t : Term), ∃ t', isNF t' ∧ t ~>* t' := by
-  sorry
+  intro t
+  by_cases h : isNF t
+  case pos =>
+    exists t
+    constructor
+    · trivial
+    · constructor
+  case neg =>
+    rw [isNF, Classical.not_forall_not] at h
+    let ⟨t', st⟩ := h
+    let ⟨t₀, ⟨t₀_nf, t'_t₀⟩⟩ := termination t'
+    exists t₀
+    constructor
+    · trivial
+    · constructor <;> assumption
+decreasing_by
+  rename_i a
+  clear a
+  induction st <;> grind [isNF]
